formal/isabelle/Jobs.thy
@@ -78,7 +78,13 @@ lemma b_lock_2048: "(2048::nat) * 24 = 49152"
 lemma g17_under_one_pct: "100 * ((3047::nat) - 3034) < 3047"
   by simp
 
-lemma g22_under_one_pct: "100 * ((13359::nat) - 13261) < 13359"
+lemma g22_under_one_pct: "100 * ((13359::nat) - 13270) < 13359"
+  by simp
+
+lemma g23_under_one_pct: "100 * ((13344::nat) - 13294) < 13344"
+  by simp
+
+lemma b_lock_119: "(119::nat) * 24 = 2856"
   by simp
 
 lemma living_jobs_surface:
@@ -86,8 +92,10 @@ lemma living_jobs_surface:
    \<and> (100003::nat) - 1 = 2 * 3 * 7 * 2381
    \<and> (8::nat) * 3 = 24
    \<and> (2048::nat) * 24 = 49152
+   \<and> (119::nat) * 24 = 2856
    \<and> 100 * ((3047::nat) - 3034) < 3047
-   \<and> 100 * ((13359::nat) - 13261) < 13359"
+   \<and> 100 * ((13359::nat) - 13270) < 13359
+   \<and> 100 * ((13344::nat) - 13294) < 13344"
   by simp
 
 end
